Work in progress on evaluation proofs.

src/Marlowe/Proof/Evaluation.lean
@@ -1,53 +1,135 @@
 
 
+import Marlowe.Language
+import Marlowe.Primitives
 import Marlowe.Semantics
 
 
 namespace Marlowe.Proof
 
 
-open Marlowe.Semantics (divide)
+open Marlowe.Language.Contract
+open Marlowe.Language.State
+open Marlowe.Primitives (Integer integer)
+open Marlowe.Semantics (evaluate observe)
 
 
-example : divide    0    0  =  0 := rfl
-example : divide    0    6  =  0 := rfl
-example : divide   12    0  =  0 := rfl
-example : divide   12    6  =  2 := rfl
-example : divide   13    6  =  2 := rfl
-example : divide   14    6  =  2 := rfl
-example : divide   15    6  =  2 := rfl
-example : divide   16    6  =  3 := rfl
-example : divide   17    6  =  3 := rfl
-example : divide   18    6  =  3 := rfl
-example : divide   19    6  =  3 := rfl
-example : divide   20    6  =  3 := rfl
-example : divide   21    6  =  4 := rfl
-example : divide   22    6  =  4 := rfl
-example : divide   23    6  =  4 := rfl
-example : divide   24    6  =  4 := rfl
-example : divide    0  (-6) =  0 := rfl
-example : divide (-12)   0  =  0 := rfl
-example : divide   12  (-6) = -2 := rfl
-example : divide (-13)   6  = -2 := rfl
-example : divide   14  (-6) = -2 := rfl
-example : divide (-15)   6  = -2 := rfl
-example : divide   16  (-6) = -3 := rfl
-example : divide (-17)   6  = -3 := rfl
-example : divide   18  (-6) = -3 := rfl
-example : divide (-19)   6  = -3 := rfl
-example : divide   20  (-6) = -3 := rfl
-example : divide (-21)   6  = -4 := rfl
-example : divide   22  (-6) = -4 := rfl
-example : divide (-23)   6  = -4 := rfl
-example : divide   24  (-6) = -4 := rfl
-example : divide    9    1  =  9 := rfl
-example : divide ( -9)   1  = -9 := rfl
+variable (e : Environment)
+variable (s : State)
+
+variable (x y : Value)
+variable (x' y' : Int)
+
+variable (hx : evaluate e s x = x')
+variable (hy : evaluate e s y = y')
+
+variable (a : Observation)
+variable (a' : Bool)
+
+variable (ha : observe e s a = a')
+
+variable (c : ChoiceIdT)
 
 
-theorem divide_by_one (x : Int) : divide x 1 = x :=
-  match x with
-    | 0 => by rfl
-    | _ => sorry
+-- theorem evaluate_money
+
+
+theorem evaluate_constant (h : x' = x''.toInt) : evaluate e s (Constant x'') = x' :=
+  by simp [evaluate, h]
+
+#check evaluate_constant
+
+
+theorem evaluate_neg :  evaluate e s (NegValue x) = - x' :=
+  by simp [evaluate, hx]
+
+#check evaluate_neg
+
+
+theorem evaluate_add : evaluate e s (AddValue x y) = x' + y' :=
+  by simp [evaluate, hx, hy]
+
+#check evaluate_add
+
+
+theorem evaluate_sub : evaluate e s (SubValue x y) = x' - y' :=
+  by simp [evaluate, hx, hy]
+
+#check evaluate_sub
+
+
+theorem evaluate_mul : evaluate e s (MulValue x y) = x' * y' :=
+  by simp [evaluate, hx, hy]
+
+#check evaluate_mul
+
+
+private def check_div (m n k : Int) : Prop :=
+  evaluate e s (DivValue (Constant $ integer m) (Constant $ integer n)) =  k
+
+example : check_div e s    0    0    0  := by simp [evaluate, check_div]
+example : check_div e s    0    6    0  := by simp [evaluate, check_div]
+example : check_div e s   12    0    0  := by simp [evaluate, check_div]
+example : check_div e s   12    6    2  := by simp [evaluate, check_div]
+example : check_div e s   13    6    2  := by simp [evaluate, check_div]
+example : check_div e s   14    6    2  := by simp [evaluate, check_div]
+example : check_div e s   15    6    2  := by simp [evaluate, check_div]
+example : check_div e s   16    6    3  := by simp [evaluate, check_div]
+example : check_div e s   17    6    3  := by simp [evaluate, check_div]
+example : check_div e s   18    6    3  := by simp [evaluate, check_div]
+example : check_div e s   19    6    3  := by simp [evaluate, check_div]
+example : check_div e s   20    6    3  := by simp [evaluate, check_div]
+example : check_div e s   21    6    4  := by simp [evaluate, check_div]
+example : check_div e s   22    6    4  := by simp [evaluate, check_div]
+example : check_div e s   23    6    4  := by simp [evaluate, check_div]
+example : check_div e s   24    6    4  := by simp [evaluate, check_div]
+example : check_div e s    0  (-6)   0  := by simp [evaluate, check_div]
+example : check_div e s (-12)   0    0  := by simp [evaluate, check_div]
+example : check_div e s   12  (-6) (-2) := by simp [evaluate, check_div]
+example : check_div e s (-13)   6  (-2) := by simp [evaluate, check_div]
+example : check_div e s   14  (-6) (-2) := by simp [evaluate, check_div]
+example : check_div e s (-15)   6  (-2) := by simp [evaluate, check_div]
+example : check_div e s   16  (-6) (-3) := by simp [evaluate, check_div]
+example : check_div e s (-17)   6  (-3) := by simp [evaluate, check_div]
+example : check_div e s   18  (-6) (-3) := by simp [evaluate, check_div]
+example : check_div e s (-19)   6  (-3) := by simp [evaluate, check_div]
+example : check_div e s   20  (-6) (-3) := by simp [evaluate, check_div]
+example : check_div e s (-21)   6  (-4) := by simp [evaluate, check_div]
+example : check_div e s   22  (-6) (-4) := by simp [evaluate, check_div]
+example : check_div e s (-23)   6  (-4) := by simp [evaluate, check_div]
+example : check_div e s   24  (-6) (-4) := by simp [evaluate, check_div]
+example : check_div e s    9    1  ( 9) := by simp [evaluate, check_div]
+example : check_div e s ( -9)   1  (-9) := by simp [evaluate, check_div]
+
+
+theorem evaluate_scale (m n : Integer) : evaluate e s (Scale m n x) = evaluate e s (DivValue (MulValue x (Constant m)) (Constant n)) :=
+  by simp [evaluate, hx]
+
+#check evaluate_scale
+
+
+-- theorem evaluate_choice
+
+
+theorem evaluate_start : evaluate e s TimeIntervalStart = e.timeInterval.fst.toInt :=
+  by simp [evaluate]
+
+#check evaluate_start
+
+
+theorem evaluate_end : evaluate e s TimeIntervalEnd = e.timeInterval.snd.toInt :=
+  by simp [evaluate]
+
+#check evaluate_end
+
+
+-- theorem evaluate_use (h : s.boundValues.contains v)
+
+
+theorem evaluate_cond : evaluate e s (Cond a x y) = if a' then x' else y' :=
+  by simp [evaluate, ha, hx, hy]
+
+#check evaluate_cond
 
 
 end Marlowe.Proof
